LeanFixpoint/VCG/STLC/Soundness.lean
@@ -17,18 +17,328 @@ open STLC
 
 theorem sub_sound (κ : KEnv) (Γ : TEnv) (s t : Ty) (c : Constraint) :
     sub s t = some c → Entail κ Γ (c κ) → Subtyp κ Γ s t := by
-  sorry
+  intro hsub hent
+  match s, t with
+  | .refine .int r1, .refine .int r2 =>
+    simp_all [sub]
+    apply Subtyp.refine
+    simp [Refinement.subImp, Formula.interp, Refinement.interp] at *
+    intro ρ hm n hf
+    have := hent ρ hm
+    rw [←hsub] at this
+    apply this
+    assumption
+  | .refine .bool r1, .refine .bool r2 =>
+    simp_all [sub]
+    apply Subtyp.refine
+    simp [Refinement.subImp, Formula.interp, Refinement.interp] at *
+    intro ρ hm
+    have h := hent ρ hm ; rw [←hsub] at h
+    obtain ⟨hl, hr⟩ := h
+    and_intros
+    · apply hl
+    · apply hr
+  | .arrow s1 t1, .arrow s2 t2 =>
+    simp_all [sub]
+    obtain ⟨c₁, hc₁⟩ : ∃ c₁, sub s2 s1 = some c₁ := by grind
+    obtain ⟨c₂, hc₂⟩ : ∃ c₂, sub (t1.openVar 0 (EVar.fresh (s1.fv ++ (s2.fv ++ (t1.fv ++ t2.fv)))))
+                                   (t2.openVar 0 (EVar.fresh (s1.fv ++ (s2.fv ++ (t1.fv ++ t2.fv))))) = some c₂ := by grind
+    rw [hc₁, hc₂] at hsub ; simp at hsub
+    apply Subtyp.arrow (x := EVar.fresh (s1.fv ++ (s2.fv ++ (t1.fv ++ t2.fv))))
+    · have h := sub_sound κ Γ s2 s1 c₁ hc₁
+      simp at h
+      rw [←hsub] at hent
+      exact h fun ρ hm => (hent ρ hm).1
+    · apply EVar.fresh_not_mem
+    · cases s2 with
+      | refine b r => cases b with
+        | int =>
+          simp_all
+          apply sub_sound _ _ _ _ c₂ hc₂
+          intro ρ hm ; simp_all
+          rw [←hsub] at hent
+          have := (hent ρ hm.2).2 (ρ.ints _) hm.1
+          simp_all
+        | bool =>
+          simp_all
+          apply sub_sound _ _ _ _ c₂ hc₂
+          intro ρ hm ; simp_all
+          rw [←hsub] at hent
+          have hb := (hent ρ hm.2).2
+          by_cases h : ρ.bools (EVar.fresh (s1.fv ++ ((Ty.refine Base.bool r).fv ++ (t1.fv ++ t2.fv)))) = false
+          · simp at h ; rw [h] at hm
+            have := hb.1 hm.1
+            have h' : (fun y => !decide (EVar.fresh (s1.fv ++ ((Ty.refine Base.bool r).fv ++ (t1.fv ++ t2.fv))) = y) && ρ.bools y) = ρ.bools := by
+              funext ; grind
+            rw [h'] at this ; simp_all
+          · simp at h ; rw [h] at hm
+            have := hb.2 hm.1
+            have h' : (fun y => decide (EVar.fresh (s1.fv ++ ((Ty.refine Base.bool r).fv ++ (t1.fv ++ t2.fv))) = y) || ρ.bools y) = ρ.bools := by
+              funext ; grind
+            rw [h'] at this ; simp_all
+      | arrow a1 a2 =>
+        simp_all
+        apply sub_sound _ _ _ _ c₂ hc₂
+        intro ρ hm ; simp at hm
+        rw [←hsub] at hent
+        exact (hent ρ hm).2
+  | .refine _ _ , .arrow _ _ | .arrow _ _, .refine _ _ | .refine .int _, .refine .bool _ | .refine .bool _, .refine .int _=>
+    simp_all [sub]
+  termination_by s.skel + t.skel
 
 /-! ## Synth / Check soundness (mutual) -/
 
 mutual
   theorem synth_sound (κ : KEnv) (Γ : TEnv) (e : Exp) (c : Constraint) (t : Ty) :
       synth Γ e = some (c, t) → Entail κ Γ (c κ) → Synth κ Γ e t := by
-    sorry
+    intro hsynth hent
+    match e with
+    | .bvar i =>
+      simp_all [synth]
+    | .fvar x =>
+      simp_all [synth]
+      rcases hsynth with ⟨t', ⟨hl, hc, hs⟩⟩
+      match t' with
+      | .refine .int r | .refine .bool r =>
+        simp_all ; rw [←hs, ←self]
+        constructor
+        assumption
+      | .arrow _ _ =>
+        simp_all ; rw [←hs, ←self] ; rw [←hs] at hl
+        constructor ; assumption
+    | .iconst i | .bconst b =>
+      simp_all [synth]
+      rw [←hsynth.2]
+      constructor
+    | .lam e | .letin e1 e2 | .and e1 e2 | .not e | .ite _ _ _  =>
+      simp_all [synth]
+    | .app e1 (.fvar y) =>
+      simp_all [synth]
+      obtain ⟨c1, s', t', hse⟩ : ∃ c s t, synth Γ e1 = some (c, .arrow s t) := by grind
+      obtain ⟨c2, hy⟩ : ∃ c, check Γ (.fvar y) s' = some c := by grind
+      simp_all
+      rw [← hsynth.2]
+      constructor <;>
+      rw [←hsynth.1] at hent
+      · exact synth_sound κ Γ e1 c1 _ hse fun ρ hm => (hent ρ hm).1
+      · exact check_sound κ Γ (.fvar y) s' c2 hy fun ρ hm => (hent ρ hm).2
+    | .ann e1 t' =>
+      simp_all [synth]
+      obtain ⟨c', hc⟩ : ∃ c, check Γ e1 t' = some c := by grind
+      simp_all
+      exact Synth.ann (check_sound κ Γ e1 t c hc hent)
+    | .leq (.fvar x) (.fvar y) | .add (.fvar x) (.fvar y) =>
+      simp_all [synth]
+      obtain ⟨a, b, ha, hb⟩ : ∃ a b, List.lookup x Γ = some (.refine .int a) ∧
+          List.lookup y Γ = some (.refine .int b) := by grind
+      simp_all
+      rw [←hsynth.2]
+      constructor <;> assumption
+    | (.add (.add _ _) _) | (.add (.leq _ _) _) | (.add (.and _ _) _) | (.add (.ann _ _) _) | (.add (.app _ _) _)
+    | (.add (.ite _ _ _) _) | (.add (.not _) _) | (.add (.letin _ _) _) | (.add (.lam _) _) | (.add (.bconst _) _)
+    | (.add (.iconst _) _) | (.add (.fvar _) (.add _ _)) | (.add (.fvar _) (.ite _ _ _)) | (.add (.fvar _) (.leq _ _))
+    | (.add (.fvar _) (.not _)) | (.add (.fvar _) (.and _ _)) | (.add (.fvar _) (.ann _ _)) | (.add (.fvar _) (.app _ _))
+    | (.add (.fvar _) (.letin _ _)) | (.add (.fvar _) (.lam _)) | (.add (.fvar _) (.bconst _)) | (.add (.fvar _) (.iconst _))
+    | (.add (.fvar _) (.bvar _)) | (.add (.bvar _) _) | (.leq (.add _ _) _) | (.leq (.ite _ _ _) _) | (.leq (.leq _ _) _)
+    | (.leq (.not _) _) | (.leq (.and _ _) _) | (.leq (.ann _ _) _) | (.leq (.app _ _) _) | (.leq (.letin _ _) _) | (.leq (.lam _) _)
+    | (.leq (.bconst _) _) | (.leq (.iconst _) _) | (.leq (.fvar _) (.add _ _)) | (.leq (.fvar _) (.ite _ _ _)) | (.leq (.fvar _) (.leq _ _))
+    | (.leq (.fvar _) (.not _)) | (.leq (.fvar _) (.and _ _)) | (.leq (.fvar _) (.ann _ _)) | (.leq (.fvar _) (.app _ _))
+    | (.leq (.fvar _) (.letin _ _)) | (.leq (.fvar _) (.lam _)) | (.leq (.fvar _) (.bconst _)) | (.leq (.fvar _) (.iconst _))
+    | (.leq (.fvar _) (.bvar _)) | (.leq (.bvar _) _) | (.app _ (.add _ _)) | (.app _ (.ite _ _ _)) | (.app _ (.leq _ _)) | (.app _ (.not _))
+    | (.app _ (.and _ _)) | (.app _ (.ann _ _)) | (.app _ (.app _ _)) | (.app _ (.letin _ _)) | (.app _ (.lam _)) | (.app _ (.bconst _))
+    | (.app _ (.iconst _)) | (.app _ (.bvar _))
+      => simp_all [synth]
+  termination_by 2*e.skel
 
   theorem check_sound (κ : KEnv) (Γ : TEnv) (e : Exp) (t : Ty) (c : Constraint) :
       check Γ e t = some c → Entail κ Γ (c κ) → Check κ Γ e t := by
-    sorry
+    intro hcheck hent
+    match e with
+    | .bvar i =>
+      simp_all [check]
+      obtain ⟨c₁, s', hc₁⟩ : ∃ c₁ s, synth Γ (.bvar i) = some (c₁, s) := by grind
+      simp_all
+      obtain ⟨c₂, hc₂⟩ : ∃ c₂, sub s' t = some c₂ := by grind
+      simp_all ; rw [←hcheck] at hent
+      exact Check.sub (synth_sound κ Γ _ _ _ hc₁ fun ρ hm => (hent ρ hm).1)
+                      (sub_sound _ _ _ _ _ hc₂ fun ρ hm => (hent ρ hm).2)
+    | .fvar x =>
+      simp_all [check]
+      obtain ⟨c₁, s', hc₁⟩ : ∃ c₁ s, synth Γ (.fvar x) = some (c₁, s) := by grind
+      simp_all
+      obtain ⟨c₂, hc₂⟩ : ∃ c₂, sub s' t = some c₂ := by grind
+      simp_all ; rw [←hcheck] at hent
+      exact Check.sub (synth_sound κ Γ _ _ _ hc₁ fun ρ hm => (hent ρ hm).1)
+                      (sub_sound _ _ _ _ _ hc₂ fun ρ hm => (hent ρ hm).2)
+    | .iconst i =>
+      simp_all [check]
+      obtain ⟨c₁, s', hc₁⟩ : ∃ c₁ s, synth Γ (.iconst i) = some (c₁, s) := by grind
+      simp_all
+      obtain ⟨c₂, hc₂⟩ : ∃ c₂, sub s' t = some c₂ := by grind
+      simp_all ; rw [←hcheck] at hent
+      exact Check.sub (synth_sound κ Γ _ _ _ hc₁ fun ρ hm => (hent ρ hm).1)
+                      (sub_sound _ _ _ _ _ hc₂ fun ρ hm => (hent ρ hm).2)
+    | .bconst b =>
+      simp_all [check]
+      obtain ⟨c₁, s', hc₁⟩ : ∃ c₁ s, synth Γ (.bconst b) = some (c₁, s) := by grind
+      simp_all
+      obtain ⟨c₂, hc₂⟩ : ∃ c₂, sub s' t = some c₂ := by grind
+      simp_all ; rw [←hcheck] at hent
+      exact Check.sub (synth_sound κ Γ _ _ _ hc₁ fun ρ hm => (hent ρ hm).1)
+                      (sub_sound _ _ _ _ _ hc₂ fun ρ hm => (hent ρ hm).2)
+    | .add e1 e2 =>
+      simp_all [check]
+      obtain ⟨c₁, s', hc₁⟩ : ∃ c₁ s, synth Γ (.add e1 e2) = some (c₁, s) := by grind
+      simp_all
+      obtain ⟨c₂, hc₂⟩ : ∃ c₂, sub s' t = some c₂ := by grind
+      simp_all ; rw [←hcheck] at hent
+      exact Check.sub (synth_sound κ Γ _ _ _ hc₁ fun ρ hm => (hent ρ hm).1)
+                      (sub_sound _ _ _ _ _ hc₂ fun ρ hm => (hent ρ hm).2)
+    | .ite (.fvar cn) bt bf =>
+      simp_all [check]
+      obtain ⟨r, hr⟩ : ∃ r, List.lookup cn Γ = some (.refine .bool r) := by grind
+      simp_all
+      obtain ⟨c₁, c₂, hc₁, hc₂⟩ : ∃ c₁ c₂,
+          (check ((cn, Ty.refine Base.bool { fmla := r.fmla.and (Formula.eqB (Term.fvar Base.bool nuName) (Term.const Base.bool true)) }) :: Γ) bt t = some c₁) ∧
+          (check ((cn, Ty.refine Base.bool { fmla := r.fmla.and (Formula.eqB (Term.fvar Base.bool nuName) (Term.const Base.bool false)) }) :: Γ) bf t = some c₂) := by
+        grind
+      simp_all
+      apply Check.ite
+      assumption
+      apply check_sound _ _ _ _ _ hc₁
+      intro ρ hm
+      rw [←hcheck] at hent
+      have := hent ρ hm.2
+      simp_all
+      by_cases h : (ρ.bools cn) = false
+      · simp at h ; rw [h] at hm
+        have := (hent ρ hm.2).1.1 hm.1
+        have h' : (fun y => !decide (cn = y) && ρ.bools y) = ρ.bools := by grind
+        rw [h'] at this ; simp_all
+      · simp at h ; rw [h] at hm
+        have := (hent ρ hm.2).1.2 hm.1
+        have h' : (fun y => decide (cn = y) || ρ.bools y) = ρ.bools := by grind
+        rw [h'] at this ; simp_all
+
+      apply check_sound _ _ _ _ _ hc₂
+      intro ρ hm
+      rw [←hcheck] at hent
+      have := hent ρ hm.2
+      simp_all
+      by_cases h : (ρ.bools cn) = false
+      · simp at h ; rw [h] at hm
+        have := (hent ρ hm.2).2.1 hm.1
+        have h' : (fun y => !decide (cn = y) && ρ.bools y) = ρ.bools := by grind
+        rw [h'] at this ; simp_all
+      · simp at h ; rw [h] at hm
+        have := (hent ρ hm.2).2.2 hm.1
+        have h' : (fun y => decide (cn = y) || ρ.bools y) = ρ.bools := by grind
+        rw [h'] at this ; simp_all
+    | .lam e =>
+      match t with
+      | .refine _ r =>
+        simp_all [check, synth]
+      | .arrow s1 t1 =>
+        simp_all [check]
+        obtain ⟨c₁, hc₁⟩ : ∃ c₁, check ((EVar.fresh (TEnv.dom Γ ++ (e.fv ++ t1.fv)), s1) :: Γ)
+            (Exp.openVar 0 (EVar.fresh (TEnv.dom Γ ++ (e.fv ++ t1.fv))) e)
+            (Ty.openVar 0 (EVar.fresh (TEnv.dom Γ ++ (e.fv ++ t1.fv))) t1) = some c₁ := by grind
+        simp_all
+        apply Check.lam (x := EVar.fresh (Γ.dom ++ (e.fv ++ t1.fv)))
+        apply EVar.fresh_not_mem
+        apply check_sound _ _ _ _ _ hc₁
+        intro ρ hm
+        rw [←hcheck] at hent
+        simp [implyBind] at hent
+        match s1 with
+        | .refine .int r =>
+          have := hent ρ hm.2 (ρ.ints (EVar.fresh (Γ.dom ++ (e.fv ++ t1.fv)))) hm.1
+          simp_all
+        | .refine .bool r =>
+          simp_all
+          have := hent ρ hm.2
+          by_cases h : (ρ.bools (EVar.fresh (Γ.dom ++ (e.fv ++ t1.fv)))) = false
+          · simp at h ; rw [h] at hm
+            have := hent ρ hm.2
+            have h' : (fun y => !decide (EVar.fresh (Γ.dom ++ (e.fv ++ t1.fv)) = y) && ρ.bools y) = ρ.bools := by
+              funext ; grind
+            rw [h'] at this ; simp_all
+          · simp at h ; rw [h] at hm
+            have := this.2 hm.1
+            have h' : (fun y => decide (EVar.fresh (Γ.dom ++ (e.fv ++ t1.fv)) = y) || ρ.bools y) = ρ.bools := by
+              funext ; grind
+            rw [h'] at this ; simp_all
+        | .arrow s1' s2' =>
+          simp_all
+    | .letin e1 e2 =>
+      simp_all [check]
+      obtain ⟨c₁, s, hc₁⟩ : ∃ c₁ s, synth Γ e1 = some (c₁, s) := by grind
+      simp_all
+      obtain ⟨c₂, hc₂⟩ : ∃ c₂, check ((EVar.fresh (Γ.dom ++ (e2.fv ++ t.fv)), s) :: Γ)
+          (Exp.openVar 0 (EVar.fresh (Γ.dom ++ (e2.fv ++ t.fv))) e2) t = some c₂ := by grind
+      simp_all
+      rw [←hcheck] at hent
+      apply Check.letin (x := EVar.fresh (Γ.dom ++ (e2.fv ++ t.fv)))
+      apply synth_sound _ _ _ _ _ hc₁
+      intro ρ hm
+      exact (hent ρ hm).1
+      rw [List.append_assoc]
+      apply EVar.fresh_not_mem
+      apply check_sound _ _ _ _ _ hc₂
+      intro ρ hm
+      match s with
+      | .refine .int r =>
+        have := (hent ρ hm.2).2 (ρ.ints (EVar.fresh (Γ.dom ++ (e2.fv ++ t.fv))))
+        simp_all
+      | .refine .bool r =>
+        simp_all
+        by_cases h : (ρ.bools (EVar.fresh (Γ.dom ++ (e2.fv ++ t.fv)))) = false
+        · simp at h ; rw [h] at hm
+          have := (hent ρ hm.2).2.1 hm.1
+          have h' : (fun y => !decide (EVar.fresh (Γ.dom ++ (e2.fv ++ t.fv)) = y) && ρ.bools y) = ρ.bools := by grind
+          simp_all
+        · simp at h ; rw [h] at hm
+          have := (hent ρ hm.2).2.2 hm.1
+          have h' : (fun y => decide (EVar.fresh (Γ.dom ++ (e2.fv ++ t.fv)) = y) || ρ.bools y) = ρ.bools := by grind
+          simp_all
+      | .arrow s₁ s₂ =>
+        simp_all
+    | .leq (.fvar x) (.fvar y) =>
+      simp_all [check]
+      obtain ⟨c₁, s, hc₁⟩ : ∃ c₁ s, synth Γ ((Exp.fvar x).leq (Exp.fvar y)) = some (c₁, s) := by grind
+      obtain ⟨c₂, hc₂⟩ : ∃ c₂, sub s t = some c₂ := by grind
+      simp_all ; rw [←hcheck] at hent
+      exact Check.sub (synth_sound _ _ _ _ _ hc₁ fun ρ hm => (hent ρ hm).1)
+                      (sub_sound _ _ _ _ _ hc₂ fun ρ hm => (hent ρ hm).2)
+    | .ann e t' =>
+      simp_all [check]
+      obtain ⟨c₁, s, hc₁⟩ : ∃ c₁ s, synth Γ (.ann e t') = some (c₁, s) := by grind
+      obtain ⟨c₂, hc₂⟩ : ∃ c₂, sub s t = some c₂ := by grind
+      simp_all ; rw [←hcheck] at hent
+      exact Check.sub (synth_sound _ _ _ _ _ hc₁ fun ρ hm => (hent ρ hm).1)
+                      (sub_sound _ _ _ _ _ hc₂ fun ρ hm => (hent ρ hm).2)
+    | .app e1 (.fvar y) =>
+      simp_all [check]
+      obtain ⟨c₁, s, hc₁⟩ : ∃ c₁ s, synth Γ (.app e1 (.fvar y)) = some (c₁, s) := by grind
+      obtain ⟨c₂, hc₂⟩ : ∃ c₂, sub s t = some c₂ := by grind
+      simp_all ; rw [←hcheck] at hent
+      exact Check.sub (synth_sound _ _ _ _ _ hc₁ fun ρ hm => (hent ρ hm).1)
+                      (sub_sound _ _ _ _ _ hc₂ fun ρ hm => (hent ρ hm).2)
+    | (.ite (.add _ _) _ _) | (.ite (.ite _ _ _) _ _) | (.ite (.leq _ _) _ _) | (.ite (.not _) _ _)
+    | (.ite (.and _ _) _ _) | (.ite (.ann _ _) _ _) | (.ite (.app _ _) _ _) | (.ite (.letin _ _) _ _)
+    | (.ite (.lam _) _ _) | (.ite (.bconst true) _ _) | (.ite (.bconst false) _ _)
+    | (.ite (.iconst _) _ _) | (.ite (.bvar _) _ _) | (.not _) | (.and _ _)
+    | (.leq (.add _ _) _) | (.leq (.ite _ _ _) _) | (.leq (.leq _ _) _) | (.leq (.not _) _)
+    | (.leq (.and _ _) _) | (.leq (.ann _ _) _) | (.leq (.app _ _) _) | (.leq (.letin _ _) _)
+    | (.leq (.lam _) _) | (.leq (.bconst _) _) | (.leq (.iconst _) _) | (.leq (.fvar _) (.add _ _))
+    | (.leq (.fvar _) (.ite _ _ _)) | (.leq (.fvar _) (.leq _ _)) | (.leq (.fvar _) (.not _)) | (.leq (.fvar _) (.and _ _))
+    | (.leq (.fvar _) (.ann _ _)) | (.leq (.fvar _) (.app _ _)) | (.leq (.fvar _) (.letin _ _)) | (.leq (.fvar _) (.lam _))
+    | (.leq (.fvar _) (.bconst _)) | (.leq (.fvar _) (.iconst _)) | (.leq (.fvar _) (.bvar _)) | (.leq (.bvar _) _)
+    | (.app _ (.add _ _)) | (.app _ (.ite _ _ _)) | (.app _ (.leq _ _)) | (.app _ (.not _))
+    | (.app _ (.and _ _)) | (.app _ (.ann _ _)) | (.app _ (.app _ _)) | (.app _ (.letin _ _)) | (.app _ (.lam _)) | (.app _ (.bconst _))
+    | (.app _ (.iconst _)) | (.app _ (.bvar _))=>
+      simp_all [check, synth]
+  termination_by 2 * e.skel + 1
 end
 
 /-! ## Bidirectional → declarative -/
@@ -49,9 +359,8 @@ mutual
     intro h
     match h with
     | .sub hsy hsub        => exact .sub (synth_to_hastype hsy) hsub
-    | .lam L hck           => exact .lam L (fun x hx => check_to_hastype (hck x hx))
-    | .letin L hsy hck     =>
-        exact .letin L (synth_to_hastype hsy) (fun x hx => check_to_hastype (hck x hx))
+    | .lam xf hck           => exact .lam xf (check_to_hastype hck)
+    | .letin hsy xf hck     => exact .letin (synth_to_hastype hsy) xf (check_to_hastype hck)
     | .ite hlk hck1 hck2   =>
         exact .ite hlk (check_to_hastype hck1) (check_to_hastype hck2)
 end
